QHC-6: Fixing types

FY/Logic.v
@@ -20,15 +20,15 @@ Open Scope hoare_spec_scope.
 Notation "P <<->> Q" :=
   (P ->> Q /\ Q ->> P) (at level 80) : hoare_spec_scope.
 
-Definition Aexp : Type := state -> R.
+Definition Aexp : Type := state -> nat.
 Definition assert_of_Prop (P : Prop) : Assertion := fun _ => P.
-Definition Aexp_of_real (n : R) : Aexp := fun _ => n.
+Definition Aexp_of_number (n : nat) : Aexp := fun _ => n.
 Definition Aexp_of_aexp (a : arith_exp) : Aexp := fun st => aeval st a.
 Coercion assert_of_Prop : Sortclass >-> Assertion.
-Coercion Aexp_of_real : R >-> Aexp.
+Coercion Aexp_of_number : nat >-> Aexp.
 Coercion Aexp_of_aexp : arith_exp >-> Aexp.
 Arguments assert_of_Prop /.
-Arguments Aexp_of_real /.
+Arguments Aexp_of_number /.
 Arguments Aexp_of_aexp /.
 Declare Scope assertion_scope.
 Bind Scope assertion_scope with Assertion.
@@ -51,10 +51,10 @@ Notation "a + b" := (fun st => mkAexp a st + mkAexp b st) : assertion_scope.
 Notation "a - b" := (fun st => mkAexp a st - mkAexp b st) : assertion_scope.
 Notation "a * b" := (fun st => mkAexp a st * mkAexp b st) : assertion_scope.
 
-Definition ap {X} (f : R -> X) (x : Aexp) :=
+Definition ap {X} (f : nat -> X) (x : Aexp) :=
   fun st => f (x st).
 
-Definition ap2 {X} (f : R -> R -> X) (x : Aexp) (y : Aexp) (st : state) :=
+Definition ap2 {X} (f : nat -> nat -> X) (x : Aexp) (y : Aexp) (st : state) :=
   f (x st) (y st).
 
 Definition hoare_triple
@@ -135,7 +135,7 @@ Ltac assn_auto :=
   try (unfold "->>", assn_sub, t_update;
        intros; simpl in *; lia). (* as in example 2 *)
 
-Example hoare_asgn_example3 : forall (a:arith_exp) (n:R),
+Example hoare_asgn_example3 : forall (a:arith_exp) (n:nat),
   {{a = n}}
   X := a; skip
   {{X = n}}.
@@ -150,7 +150,7 @@ Proof.
 Admitted.
 
 Definition bassn b : Assertion :=
-  fun st => (beval st b = True).
+  fun st => (beval st b = true).
 
 Coercion bassn : bool_exp >-> Assertion.
 
@@ -158,12 +158,12 @@ Arguments bassn /.
 Hint Unfold bassn : core.
 
 Lemma bexp_eval_true : forall b st,
-  beval st b = True -> (bassn b) st.
+  beval st b = true -> (bassn b) st.
 Proof. auto. Qed.
 
 Lemma bexp_eval_false : forall b st,
-  beval st b = False -> ~ ((bassn b) st).
-Proof. (*congruence*) Admitted.
+  beval st b = false -> ~ ((bassn b) st).
+Proof. congruence. Qed.
 
 Hint Resolve bexp_eval_false : core.
 
@@ -182,6 +182,6 @@ Ltac assn_auto' :=
   try rewrite -> eqb_eq in *; (* for equalities *)
   auto; try lia.
 
-Lemma eqb_eq': forall (n m: nat), Nat.eqb n m = true <-> n = m.
+Lemma eqb_eq': forall (n m: nat), eq n m = True <-> n = m.
 Proof.
 Admitted.
